proof/spec/Types.ec
@@ -9,26 +9,9 @@ require import Array8.
 
 type adrs = W32.t Array8.t.
 
-clone import Subtype as NBytes with 
-   type T = W8.t list,
-   op P = fun l => size l = n
-   rename "T" as "nbytes"
-   proof inhabited by (exists (nseq n W8.zero);smt(size_nseq ge0_n))
-   proof *.
-
-clone import Subtype as LEN_N with 
-   type T = nbytes list,
-   op P = fun l => size l = len
-   rename "T" as "len_n_bytes"
-   proof inhabited by (exists (nseq len (nseq n W8.zero));smt(size_nseq ge0_len))
-   proof *.
-
-clone import Subtype as LEN1 with 
-   type T = W8.t list,
-   op P = fun l => size l = len1
-   rename "T" as "len1_bytes"
-   proof inhabited by (exists (nseq len1 W8.zero);smt(size_nseq ge0_len1))
-   proof *.
+type nbytes = W8.t list. (* size = n *)
+type len_n_bytes = nbytes list. (* list of length len, each element of length n *)
+type len1_bytes = W8.t list. (* list of length len1 *)
 
 (******************************************************************************)
 
